

Homework_1 David Cortes

Math 742

Cosella / Berger

1.2d : Prove $A \cup B = A \cup (B \cap A^c)$

I'll start with the Right-Hand Side and simplify it using the distribute law, which is stated in Theorem 1.1.4.

In set theory proofs, equality of sets is proven by double containment

$$\textcircled{i} A \cup B \subseteq A \cup (B \cap A^c) \quad \wedge \quad A \cup (B \cap A^c) \subseteq A \cup B \quad \textcircled{ii}$$

① Taking an arbitrary element $x \in A \cup B$. By definition of union:

$$x \in A \cup B \rightarrow x \in A \text{ or } x \in B$$

Now, let's consider the two cases:

$$\text{case 1: } x \in A \rightarrow x \in A \subseteq A \cup (B \cap A^c)$$

$$\text{Case 2: } x \in B \wedge x \notin A \begin{matrix} \nearrow x \in B \\ \searrow x \in A^c \end{matrix}$$

$$\text{So, } x \in B \cap A^c \rightarrow x \in A \cup (B \cap A^c)$$

In both cases, $x \in A \cup (B \cap A^c)$ thus: $A \cup B \subseteq (B \cap A^c)$

② Taking an arbitrary $x \in A \cup (B \cap A^c) \rightarrow x \in A \vee x \in (B \cap A^c)$

$$\text{case 1: } x \in A \text{ then } x \in A \cup B \quad \text{case 2: } x \in B \cap A^c \text{ then } x \in B \rightarrow x \in A \cup B$$

Again in both cases $x \in A \cup B$ thus $A \cup (B \cap A^c) \subseteq A \cup B$

• After proving the above result, prove: $P(A \cup B) = P(A) + P(B) - P(A \cap B)$

from above $A \cup B = A \cup (B \cap A^c) \rightarrow A$ and $B \cap A^c$ are disjoint $A \cap (B \cap A^c) = \emptyset$

Why? $A \cap (B \cap A^c) \rightarrow$ using associative of intersection $A \cap (B \cap A^c) = (A \cap B) \cap A^c$. so any element x in this set must satisfy all 3 conditions: $x \in A$, $x \in B$, $x \in A^c$. then by definition $(A \cap B) \cap A^c = \emptyset$

$$\text{from above, if } C \cap D = \emptyset \text{ then } P(C \cup D) = P(C) + P(D) \rightarrow P(A \cup B) = P(A) + P(B \cap A^c)$$

Rewriting $P(B \cap A^c)$, $B = (B \cap A) \cup (B \cap A^c)$ (decomposition)

$$P(B) = P(B \cap A) + P(B \cap A^c) \rightarrow P(B \cap A^c) = P(B) - P(A \cap B)$$

$$\text{Then } P(A \cup B) = P(A) + P(B \cap A^c) \\ = P(A) + P(B) - P(A \cap B)$$

1.3c De Morgan's Laws. Prove this without Venn diagrams.

$$\textcircled{i} (A \cup B)^c = \underline{A^c \cap B^c} \quad \wedge \quad \textcircled{ii} (A \cap B)^c = \underline{A^c \cup B^c}$$

$$\textcircled{i} \text{ If an } x \in (A \cup B)^c \leftrightarrow x \notin A \vee x \notin B \leftrightarrow x \in A^c \wedge x \in B^c \leftrightarrow x \in \underline{A^c \cap B^c}$$

$$\textcircled{ii} \text{ If an } x \in (A \cap B)^c \leftrightarrow x \notin A \cap B \leftrightarrow x \notin A \vee x \notin B \leftrightarrow x \in A^c \vee x \in B^c \leftrightarrow x \in \underline{A^c \cup B^c}$$

1.4/6: Prove that $F_X(x) = \frac{1}{1+e^{-x}}$, $x \in (-\infty, \infty)$ is a CDF.

Our $F_X(x)$ satisfies the conditions of theorem 1.5.3

Theorem 1.5.3 The function $F(x)$ is a CDF \iff The following 3 conditions hold:

a. $\lim_{x \rightarrow -\infty} F(x) = 0$ \wedge $\lim_{x \rightarrow \infty} F(x) = 1$ (Monotonicity)

b. $F(x)$ is a NONDECREASING function of x .

c. $F(x)$ is RIGHT continuous; that is, for every number x_0 , $\lim_{x \downarrow x_0} F(x) = F(x_0)$

outline of proof: To prove necessity, the three properties can be verified by writing F in terms of the probability function.

If $F_X(\cdot)$ is a CDF, $F_X(x) = P(X \leq x)$. Hence $\lim_{x \rightarrow \infty} P(X \leq x) = 1$ \wedge $\lim_{x \rightarrow -\infty} P(X \leq x) = 0$

$F(x)$ is nondecreasing since the set $\{x : X \leq x\}$ is nondecreasing in x .

lastly, as $x \downarrow x_0$, $P(X \leq x) \rightarrow P(X \leq x_0)$, Then $F_X(\cdot)$ is RIGHT continuous.

4.4 A PDF is defined by,

$$f(x, y) = \begin{cases} c(x+2y) : 0 < y < 1 \wedge 0 < x < 2 \\ 0 & : \text{otherwise} \end{cases}$$

a) find the value of c .

$$\int_0^2 \int_0^1 c(x+2y) dy dx = \underline{1} \text{ (the total probability)}$$

$$(y) \rightarrow \int_0^1 (x+2y) dy = (xy + y^2) \Big|_0^1 = (x+1) - (0) = x+1$$

$$(x) \rightarrow c \int_0^2 (x+1) dx = c \left(\frac{x^2}{2} + x \right) \Big|_0^2 = c((2+2) - (0)) = 4c$$

$$\underline{4c = 1} \rightarrow c = 1/4$$

b) Find the marginal distribution of X .

To find $f_X(x)$, I should integrate the joint PDF over the range of y

$$f_X(x) = \begin{cases} \int_0^1 \frac{1}{4}(x+2y) dy, \text{ we did it previously} = \frac{1}{4}(x+1), & 0 < x < 2 \\ 0 & \text{otherwise} \end{cases}$$

c) Find the joint CDF of X and Y . $= F_{XY}(x, y) = P(X \leq x, Y \leq y)$

$$P(X \leq x, Y \leq y) = \int_{-\infty}^x \int_{-\infty}^y f(v, u) dv du = \int_0^x \int_0^y \frac{1}{4}(u+2v) dv du$$

Inner Integral (w.r.t. v) $\frac{1}{4} [uv + v^2]_0^y = \frac{1}{4} (uy + y^2)$

Outer Integral (w.r.t. u) $\int_0^x \frac{1}{4} (uy + y^2) du = \frac{1}{4} [\frac{1}{2} u^2 y + uy^2]_0^x$

$$F_{XY}(x, y) = \frac{x^2 y}{8} + \frac{xy^2}{4} \quad \text{for } 0 < x < 2 \wedge 0 < y < 1$$

$$F_{XY}(x, y) = \int_{-\infty}^x \int_{-\infty}^y f(u, v) dv du = \int_0^x \int_0^1 \frac{1}{4}(u+2v) dv du = \frac{x^2}{8} + \frac{x}{4}$$

Then, the full definition of F_{XY} is

$$F_{XY}(x, y) = \begin{cases} 0 & x \leq 0 \vee y \leq 0 \\ x^2 y / 8 + xy^2 / 4 & 0 < x < 2 \wedge 0 < y < 1 \\ y/2 + y^2/2 & 2 \leq x \wedge 0 < y < 1 \\ x^2/8 + x/4 & 0 < x < 2 \wedge 1 \leq y \\ 1 & 2 \leq x \wedge 1 \leq y \end{cases}$$

d) Find the PDF of the random variable $Z = g(X+1)^2$

Apply Theorem 2.1.5 (Monotonicity) Computing derivative:

$$g'(x) = -\frac{18}{(x+1)^3} < 0 \quad \text{for } x > 0. \quad \text{So } g(x) \text{ is strictly monotone decreasing on } 0 < x < 2$$

- Find the support of Z :

Evaluate endpoints at $x=0$: $z = \frac{9}{(1)^2} = 9$ at $x=2$: $z = \frac{9}{(3)^2} = 1$

Since g is decreasing

$$1 < Z < 9$$

- Invert the transformation

Start from

$$z = \frac{9}{(x+1)^2} \quad \text{solve for } x: (x+1)^2 = \frac{9}{z} \rightarrow x+1 = \frac{3}{\sqrt{z}}$$

$$x = \frac{3}{\sqrt{z}} - 1 \quad (\text{only } + (\text{positive}) \text{ root is valid since } x+1 > 0)$$

$$\sqrt{z}$$

- Compute the Jacobian. $\frac{dx}{dz} = -\frac{3}{2} z^{-3/2} \rightarrow \frac{dx}{dz} = \frac{3}{2z^{3/2}}$

- For a monotone transformation:

$$f_Z(z) = f_X(x(z)) \left| \frac{dx}{dz} \right|$$

- substitute

compute $f_X(x(z))$ $x+1 = \frac{3}{\sqrt{z}}$

$$f_X(x) = \frac{1}{4}(x+1) = \frac{3}{4\sqrt{z}}$$

- Multiply by Jacobian $f_Z(z) = \frac{3}{4\sqrt{z}} \cdot \frac{3}{2z^{3/2}} = \frac{9}{8z^2} \rightarrow f_Z(z) = \begin{cases} \frac{9}{8z^2}, & 1 < z < 9 \\ 0 & \text{otherwise} \end{cases}$

4.10 The random pair (X, Y) has the distribution

| | X=1 | X=2 | X=3 |
|-----|----------------|---------------|----------------|
| Y=2 | $\frac{1}{12}$ | $\frac{1}{6}$ | $\frac{1}{12}$ |
| Y=3 | $\frac{1}{6}$ | 0 | $\frac{1}{6}$ |
| Y=4 | 0 | $\frac{1}{3}$ | 0 |

a) Show that X and Y are dependent. Two discrete random variables X, Y are independent if: $P(X=x, Y=y) = P(X=x)P(Y=y) \forall x, y$

Once counter example

$$P(X=2, Y=3) = 0$$

But if X and Y were independent:

$$P(X=2)P(Y=3) = \frac{1}{2} \cdot \frac{1}{3} = \frac{1}{6}$$

$$0 \neq \frac{1}{6} \rightarrow X \text{ and } Y \text{ are dependent}$$

b) Give a probability table for random variables U and V that have the same marginals as X as Y but are independent.

The distribution that satisfies $P(U=x, V=y) = P(U=x)P(V=y)$ where $U \sim X$ and $V \sim Y$ is

| | U=1 | U=2 | U=3 |
|-----|----------------|---------------|----------------|
| V=2 | $\frac{1}{12}$ | $\frac{1}{6}$ | $\frac{1}{12}$ |
| V=3 | $\frac{1}{12}$ | $\frac{1}{6}$ | $\frac{1}{12}$ |
| V=4 | $\frac{1}{12}$ | $\frac{1}{6}$ | $\frac{1}{12}$ |

Wasserman

3.10 $X \sim N(0,1)$, $Y \sim e^X$. Determine $E(Y)$ and $V(Y)$

$$E(Y) = \frac{1}{\sqrt{2\pi}} \int_{-\infty}^{\infty} e^x e^{-x^2/2} dx = \frac{1}{\sqrt{2\pi}} \int_{-\infty}^{\infty} e^{\frac{x(2-x)}{2}} dx \quad \text{let } u = x-1$$

$$\rightarrow E(Y) = \frac{1}{\sqrt{2\pi}} \int_{-\infty}^{\infty} e^{\frac{1-u^2}{2}} du = e^{1/2} \int_{-\infty}^{\infty} \frac{e^{-u^2/2}}{\sqrt{2\pi}} du = e^{1/2}$$

$$E(Y^2) = \frac{1}{\sqrt{2\pi}} \int_{-\infty}^{\infty} e^{2x - \frac{x^2}{2}} dx \quad \text{lets } u = x-2$$

$$\rightarrow E(Y^2) = \frac{1}{\sqrt{2\pi}} \int_{-\infty}^{\infty} e^2 e^{-u^2/2} du = e^2$$

$$V(Y) = E(Y^2) - E(Y)^2 = e^2 - (e^{1/2})^2 = e^2 - e$$

NO TIME TO WORK ON IT

3.19

Extra Problem:

Let X have a gamma distribution with parameters α, β .

Prove that $E(X) = \alpha\beta$ and $V(X) = \alpha\beta^2$

The Gamma PDF is defined as:

- $\alpha > 0$

- $\beta > 0$

$$f_X(x) = \frac{\beta^\alpha}{\Gamma(\alpha)\beta^\alpha} x^{\alpha-1} e^{-x/\beta} \quad \Gamma(\alpha) = \int_0^\infty t^{\alpha-1} e^{-t} dt$$

Show that: $E(X) = \alpha\beta$ and $V(X) = \alpha\beta^2$

